code/coq/aux.v
@@ -18,3 +18,11 @@ Proof. rewrite rev_cons. apply rcons_non_empty. Qed.
 Lemma leq_add:
   forall a b, a <= b -> exists c, a + c = b.
 Admitted.
+
+Lemma map_app {T:Type} {Q:Type}:
+  forall (l1: list T) l2 (f:T->Q),
+    [seq f x | x <- l1] ++ [seq f x | x <- l2] =
+    [seq f x | x <- l1 ++ l2].
+Proof.
+  induction l1; auto; intros; simpl; f_equal; auto.
+Qed.
